theories/Poly/Ctx.v
@@ -7,190 +7,177 @@ Set Strict Implicit.
 
 Module Type Context.
   Parameter iT : Type.
-  Parameter Denote : iT -> Type.
 
-  Parameter Env : list iT -> Type.
-  Parameter Env_nil : Env nil.
+  Section denoted.
+    Variable Denote : iT -> Type.
 
-  (** Dependent contexts are like [Pi]s **)
-  Parameter DCtx : forall ts : list iT, (Env ts -> Type) -> Type.
-
-  Parameter eval_Ctx : forall ts F, DCtx F -> forall x : Env ts, F x.
-
-  Parameter dpure : forall ts F, (forall x : Env ts, F x) -> @DCtx ts F.
-  Parameter dap   : forall ts F G,
-                      @DCtx ts (fun x => F x -> G x) ->
-                      @DCtx ts F ->
-                      @DCtx ts G.
-  Parameter dfmap : forall ts F G,
-                      (forall x : Env ts, F x -> G x) ->
-                      @DCtx ts F ->
-                      @DCtx ts G.
-
-  Parameter Env_weaken : forall ts ts', Env (ts ++ ts') -> Env ts.
-  Parameter Env_tl : forall t ts, Env (t :: ts) -> Env ts.
-  Parameter DCtx_weaken
-  : forall ts ts' F,
-      @DCtx ts F ->
-      @DCtx (ts ++ ts') (fun x => F (Env_weaken ts ts' x)).
+    Parameter Env : (iT -> Type) -> list iT -> Type.
+    Parameter Env_nil : Env Denote nil.
+    Parameter Env_weaken : forall ts ts', Env Denote (ts ++ ts') -> Env Denote ts.
+    Parameter Env_tl : forall t ts, Env Denote (t :: ts) -> Env Denote ts.
 
 
-  (** Quantify **)
-  Parameter Quant_DCtx
-  : forall {ks : list iT} {T : Env ks -> Type} {k : iT},
-      (forall e, (Denote k -> T e) -> T e) ->
-      @DCtx (cons k ks) (fun g => T (Env_tl g)) -> @DCtx ks T.
+    (** Dependent contexts are like [Pi]s **)
+    Parameter DCtx : forall ts : list iT, (Env Denote ts -> Type) -> Type.
 
-  Parameter Use_DCtx'
-  : forall {ks k} (m : member k ks), @DCtx ks (fun _ => Denote k).
+    Parameter eval_Ctx : forall ts F, DCtx F -> forall x : Env Denote ts, F x.
 
-  Parameter Env_get : forall k ks, member k ks -> Env ks -> Denote k.
+    Parameter dpure : forall ts F, (forall x : Env Denote ts, F x) -> @DCtx ts F.
+    Parameter dap   : forall ts F G,
+                        @DCtx ts (fun x => F x -> G x) ->
+                        @DCtx ts F ->
+                        @DCtx ts G.
+    Parameter dfmap : forall ts F G,
+                        (forall x : Env Denote ts, F x -> G x) ->
+                        @DCtx ts F ->
+                        @DCtx ts G.
 
-  Parameter Use_DCtx
-  : forall {ks k} (m : member k ks)
+    Parameter DCtx_weaken
+    : forall ts ts' F,
+        @DCtx ts F ->
+        @DCtx (ts ++ ts') (fun x => F (Env_weaken ts ts' x)).
+
+    (** Quantify **)
+    Parameter Quant_DCtx
+    : forall {ks : list iT} {T : Env Denote ks -> Type} {k : iT},
+        (forall e, (Denote k -> T e) -> T e) ->
+        @DCtx (cons k ks) (fun g => T (Env_tl g)) -> @DCtx ks T.
+
+    Parameter Use_DCtx'
+    : forall {ks k} (m : member k ks), @DCtx ks (fun _ => Denote k).
+
+    Parameter Env_get : forall k ks, member k ks -> Env Denote ks -> Denote k.
+
+    Parameter Use_DCtx
+    : forall {ks k} (m : member k ks)
              (F : Denote k -> Type) (ret : forall v, F v),
-      @DCtx ks (fun e => F (Env_get m e)).
+        @DCtx ks (fun e => F (Env_get m e)).
 
-  (** Contexts **)
-  Definition Ctx ts T : Type :=
-    @DCtx ts (fun _ => T).
+    (** Contexts **)
+    Definition Ctx ts T : Type :=
+      @DCtx ts (fun _ => T).
 
-  Definition Applicative_Ctx {ks} : Applicative (Ctx ks) :=
-  {| pure := fun _ X => dpure _ (fun _ : Env ks => X)
-   ; ap := fun (A B : Type) (f : DCtx (fun _ : Env ks => A -> B))
-         (x : DCtx (fun _ : Env ks => A)) => dap _ f x
-   |}.
+    Definition Applicative_Ctx {ks} : Applicative (Ctx ks) :=
+      {| pure := fun _ X => dpure _ (fun _ : Env Denote ks => X)
+         ; ap := fun (A B : Type) (f : DCtx (fun _ : Env Denote ks => A -> B))
+                     (x : DCtx (fun _ : Env Denote ks => A)) => dap _ f x
+      |}.
 
-  Definition Functor_Ctx {ks} : Functor (Ctx ks) :=
-  {| fmap := fun (A B : Type) (X : A -> B) (X0 : Ctx ks A) =>
-         dfmap _ (fun _ : Env ks => X) X0 |}.
+    Definition Functor_Ctx {ks} : Functor (Ctx ks) :=
+      {| fmap := fun (A B : Type) (X : A -> B) (X0 : Ctx ks A) =>
+                   dfmap _ (fun _ : Env Denote ks => X) X0 |}.
 
-  Definition Ctx_weaken ks ks' T (ctx : Ctx ks T) : Ctx (ks ++ ks') T :=
-    @DCtx_weaken ks ks' (fun _ => T) ctx.
+    Definition Ctx_weaken ks ks' T (ctx : Ctx ks T) : Ctx (ks ++ ks') T :=
+      @DCtx_weaken ks ks' (fun _ => T) ctx.
 
-  Definition Quant_Ctx (T : Type) {k : iT} {ks : list iT}
-             (Q : (Denote k -> T) -> T)
-             (ctx : Ctx (cons k ks) T)
-  : Ctx ks T :=
-    Quant_DCtx (fun _ : Env ks => Q) ctx.
+    Definition Quant_Ctx (T : Type) {k : iT} {ks : list iT}
+               (Q : (Denote k -> T) -> T)
+               (ctx : Ctx (cons k ks) T)
+    : Ctx ks T :=
+      Quant_DCtx (fun _ : Env Denote ks => Q) ctx.
 
-  Definition Use_Ctx {ks k} (m : member k ks) : Ctx ks (Denote k) :=
-    Use_DCtx' m.
+    Definition Use_Ctx {ks k} (m : member k ks) : Ctx ks (Denote k) :=
+      Use_DCtx' m.
 
-
-(*
-  (** Non-dependent contexts are just a specialization of dependent contexts **)
-
-  Parameter Applicative_Ctx : forall ks, Applicative (Ctx ks).
-  Parameter Functor_Ctx : forall ks, Functor (Ctx ks).
-
-  (** TODO: There should be a naturality property about this,
-   ** i.e. how it interacts with [ap], [pure], and [fmap]
-   **)
-  Parameter Ctx_weaken
-  : forall ks ks' T, Ctx ks T -> Ctx (ks ++ ks') T.
-*)
+  End denoted.
 
 End Context.
 
 Module Type ContextP.
   Parameter iT : Type.
-  Parameter Denote : iT -> Type.
 End ContextP.
 
-Module Type ContextBuilder (P : ContextP)
-:= Context with Definition iT := P.iT
-           with Definition Denote := P.Denote.
-
 Module ContextHList (P : ContextP)
-<: Context with Definition iT := P.iT
-          with Definition Denote := P.Denote.
+<: Context with Definition iT := P.iT.
 
   Definition iT : Type := P.iT.
-  Definition Denote : iT -> Type := P.Denote.
 
-  Definition Env : list iT -> Type := hlist Denote.
+  Section denoted.
+    Variable Denote : iT -> Type.
 
-  Definition Env_nil : Env nil := Hnil.
-  Definition Env_tl {t ts} : Env (t :: ts) -> Env ts :=
-    @hlist_tl _ _ _ _.
+    Definition Env : list iT -> Type := hlist Denote.
+
+    Definition Env_nil : Env nil := Hnil.
+    Definition Env_tl {t ts} : Env (t :: ts) -> Env ts :=
+      @hlist_tl _ _ _ _.
 
 
-  (** Dependent contexts are like [Pi]s **)
-  Definition DCtx (ts : list iT) (F : Env ts -> Type) : Type :=
-    forall env, F env.
+    (** Dependent contexts are like [Pi]s **)
+    Definition DCtx (ts : list iT) (F : Env ts -> Type) : Type :=
+      forall env, F env.
 
-  Definition eval_Ctx {ts F} (ctx : DCtx F) (e : Env ts) : F e :=
-    ctx e.
+    Definition eval_Ctx {ts F} (ctx : DCtx F) (e : Env ts) : F e :=
+      ctx e.
 
-  Definition dpure {ts F} (val : forall x : Env ts, F x) : @DCtx ts F :=
-    val.
+    Definition dpure {ts F} (val : forall x : Env ts, F x) : @DCtx ts F :=
+      val.
 
-  Definition dap {ts F G }
-             (f : @DCtx ts (fun x => F x -> G x))
-             (x : @DCtx ts F)
-  : @DCtx ts G :=
-    fun e => f e (x e).
+    Definition dap {ts F G }
+               (f : @DCtx ts (fun x => F x -> G x))
+               (x : @DCtx ts F)
+    : @DCtx ts G :=
+      fun e => f e (x e).
 
-  Definition dfmap {ts F G}
-             (f : forall x : Env ts, F x -> G x)
-             (ctx : @DCtx ts F)
-  : @DCtx ts G :=
-    fun e => f e (ctx e).
+    Definition dfmap {ts F G}
+               (f : forall x : Env ts, F x -> G x)
+               (ctx : @DCtx ts F)
+    : @DCtx ts G :=
+      fun e => f e (ctx e).
 
-  (** This operation is not valid for iterated environments! **)
-  Definition Env_weaken {ts ts'} (ctx : Env (ts ++ ts')) : Env ts :=
-    fst (hlist_split ts ts' ctx). (** This requires a weakening **)
+    (** This operation is not valid for iterated environments! **)
+    Definition Env_weaken {ts ts'} (ctx : Env (ts ++ ts')) : Env ts :=
+      fst (hlist_split ts ts' ctx). (** This requires a weakening **)
 
-  Definition DCtx_weaken {ts ts' F}
-             (ctx : @DCtx ts F)
-  : @DCtx (ts ++ ts') (fun x => F (Env_weaken x)) :=
-    fun e => ctx _.
+    Definition DCtx_weaken {ts ts' F}
+               (ctx : @DCtx ts F)
+    : @DCtx (ts ++ ts') (fun x => F (Env_weaken x)) :=
+      fun e => ctx _.
 
-  (** Quantify **)
-  Definition Quant_DCtx
-             {ks : list iT} {T : Env ks -> Type} {k : iT}
-             (Q : forall e, (Denote k -> T e) -> T e)
-             (v : @DCtx (cons k ks) (fun g => T (Env_tl g)))
-  :  @DCtx ks T :=
-    fun env => Q env (fun (x : _) => v (Hcons x env)).
+    (** Quantify **)
+    Definition Quant_DCtx
+               {ks : list iT} {T : Env ks -> Type} {k : iT}
+               (Q : forall e, (Denote k -> T e) -> T e)
+               (v : @DCtx (cons k ks) (fun g => T (Env_tl g)))
+    :  @DCtx ks T :=
+      fun env => Q env (fun (x : _) => v (Hcons x env)).
 
-  Definition Env_get {k ks} (m : member k ks) : Env ks -> Denote k :=
-    @hlist_get _ _ _ _ m.
+    Definition Env_get {k ks} (m : member k ks) : Env ks -> Denote k :=
+      @hlist_get _ _ _ _ m.
 
-  Definition Use_DCtx' {ks k} (m : member k ks)
-  : @DCtx ks (fun _ => Denote k) :=
-    fun e => hlist_get m e.
+    Definition Use_DCtx' {ks k} (m : member k ks)
+    : @DCtx ks (fun _ => Denote k) :=
+      fun e => hlist_get m e.
 
-  Definition Use_DCtx {ks k} (m : member k ks)
-             (F : Denote k -> Type) (ret : forall v, F v)
-  : @DCtx ks (fun e => F (hlist_get m e)) :=
-    fun e => ret (Env_get m e).
+    Definition Use_DCtx {ks k} (m : member k ks)
+               (F : Denote k -> Type) (ret : forall v, F v)
+    : @DCtx ks (fun e => F (hlist_get m e)) :=
+      fun e => ret (Env_get m e).
 
-  (** Contexts **)
-  Definition Ctx ts T : Type :=
-    @DCtx ts (fun _ => T).
+    (** Contexts **)
+    Definition Ctx ts T : Type :=
+      @DCtx ts (fun _ => T).
 
-  Definition Applicative_Ctx {ks} : Applicative (Ctx ks) :=
-  {| pure := fun _ X => dpure (fun _ : Env ks => X)
-   ; ap := fun (A B : Type) (f : DCtx (fun _ : Env ks => A -> B))
-         (x : DCtx (fun _ : Env ks => A)) => dap f x
-   |}.
+    Definition Applicative_Ctx {ks} : Applicative (Ctx ks) :=
+      {| pure := fun _ X => dpure (fun _ : Env ks => X)
+         ; ap := fun (A B : Type) (f : DCtx (fun _ : Env ks => A -> B))
+                     (x : DCtx (fun _ : Env ks => A)) => dap f x
+      |}.
 
-  Definition Functor_Ctx {ks} : Functor (Ctx ks) :=
-  {| fmap := fun (A B : Type) (X : A -> B) (X0 : Ctx ks A) =>
-         dfmap (fun _ : Env ks => X) X0 |}.
+    Definition Functor_Ctx {ks} : Functor (Ctx ks) :=
+      {| fmap := fun (A B : Type) (X : A -> B) (X0 : Ctx ks A) =>
+                   dfmap (fun _ : Env ks => X) X0 |}.
 
-  Definition Ctx_weaken ks ks' T (ctx : Ctx ks T) : Ctx (ks ++ ks') T :=
-    @DCtx_weaken ks ks' (fun _ => T) ctx.
+    Definition Ctx_weaken ks ks' T (ctx : Ctx ks T) : Ctx (ks ++ ks') T :=
+      @DCtx_weaken ks ks' (fun _ => T) ctx.
 
-  Definition Quant_Ctx (T : Type) {k : iT} {ks : list iT}
-             (Q : (Denote k -> T) -> T)
-             (ctx : Ctx (cons k ks) T)
-  : Ctx ks T :=
-    Quant_DCtx (fun _ : Env ks => Q) ctx.
+    Definition Quant_Ctx (T : Type) {k : iT} {ks : list iT}
+               (Q : (Denote k -> T) -> T)
+               (ctx : Ctx (cons k ks) T)
+    : Ctx ks T :=
+      Quant_DCtx (fun _ : Env ks => Q) ctx.
 
-  Definition Use_Ctx {ks k} (m : member k ks) : Ctx ks (Denote k) :=
-    Use_DCtx' m.
+    Definition Use_Ctx {ks k} (m : member k ks) : Ctx ks (Denote k) :=
+      Use_DCtx' m.
+  End denoted.
 
 End ContextHList.
